change: substs → rewrite

Logic/FirstOrder/Basic/Formula.lean
@@ -16,6 +16,8 @@ inductive Subformula (L : Language.{u}) (μ : Type v) : ℕ → Type (max u v) w
 
 abbrev Formula (L : Language.{u}) (μ : Type v) := Subformula L μ 0
 
+abbrev FormulaFin (L : Language.{u}) (n : ℕ) := Subformula L (Fin n) 0
+
 abbrev Sentence (L : Language.{u}) := Formula L Empty
 
 abbrev Subsentence (L : Language.{u}) (n : ℕ) := Subformula L Empty n
@@ -504,10 +506,10 @@ scoped syntax (name := substsHomNotation) term:max "#[" term,* "]" : term
 scoped macro_rules (kind := substsHomNotation)
   | `($p:term #[$terms:term,*]) => `((Rew.substs ![$terms,*]).hom $p)
 
-scoped syntax (name := rewriteMapHomNotation) term:max "&[" term,* "]" : term
+scoped syntax (name := rewriteHomNotation) term:max "&[" term,* "]" : term
 
-scoped macro_rules (kind := rewriteMapHomNotation)
-  | `($p:term &[$terms:term,*]) => `((Rew.rewriteMap ![$terms,*]).hom $p)
+scoped macro_rules (kind := rewriteHomNotation)
+  | `($p:term &[$terms:term,*]) => `((Rew.rewrite ![$terms,*]).hom $p)
 
 namespace Subformula
 
@@ -583,14 +585,14 @@ def qfree (p : Subformula L μ n) : Prop := p.qr = 0
   by simp[qfree]
 
 structure Operator (L : Language.{u}) (n : ℕ) where
-  sentence : Subsentence L n
+  sentence : FormulaFin L n
 
 abbrev Const (L : Language.{u}) := Operator L 0
 
 namespace Operator
 
 def operator {arity : ℕ} (o : Operator L arity) (v : Fin arity → Subterm L μ n) : Subformula L μ n :=
-  (Rew.substs v).hom (Rew.emb.hom o.sentence)
+  (Rew.rewrite v).hom ((Rew.castLE n.zero_le).hom o.sentence)
 
 def const (c : Const L) : Subformula L μ n := c.operator ![]
 
@@ -604,7 +606,6 @@ lemma operator_comp (o : Operator L k) (w : Fin k → Subterm.Operator L l) (v :
     simp[operator, comp, ←Rew.hom_comp_app]; congr 2
     ext <;> simp[Rew.comp_app]
     · congr
-    · contradiction
 
 def and {k} (o₁ o₂ : Operator L k) : Operator L k := ⟨o₁.sentence ⋏ o₂.sentence⟩
 
@@ -628,15 +629,15 @@ protected class LE (L : Language) where
 protected class Mem (L : Language) where
   mem : Subformula.Operator L 2
 
-instance [Language.Eq L] : Operator.Eq L := ⟨⟨Subformula.rel Language.Eq.eq Subterm.bvar⟩⟩
+instance [Language.Eq L] : Operator.Eq L := ⟨⟨Subformula.rel Language.Eq.eq Subterm.fvar⟩⟩
 
-instance [Language.LT L] : Operator.LT L := ⟨⟨Subformula.rel Language.LT.lt Subterm.bvar⟩⟩
+instance [Language.LT L] : Operator.LT L := ⟨⟨Subformula.rel Language.LT.lt Subterm.fvar⟩⟩
 
 instance [Operator.Eq L] [Operator.LT L] : Operator.LE L := ⟨Eq.eq.or LT.lt⟩
 
-lemma Eq.sentence_eq [L.Eq] : (@Operator.Eq.eq L _).sentence = Subformula.rel Language.Eq.eq Subterm.bvar := rfl
+lemma Eq.sentence_eq [L.Eq] : (@Operator.Eq.eq L _).sentence = Subformula.rel Language.Eq.eq Subterm.fvar := rfl
 
-lemma LT.sentence_eq [L.LT] : (@Operator.LT.lt L _).sentence = Subformula.rel Language.LT.lt Subterm.bvar := rfl
+lemma LT.sentence_eq [L.LT] : (@Operator.LT.lt L _).sentence = Subformula.rel Language.LT.lt Subterm.fvar := rfl
 
 lemma LE.def_of_Eq_of_LT [Operator.Eq L] [Operator.LT L] :
     (@Operator.LE.le L _) = Eq.eq.or LT.lt := rfl
@@ -791,6 +792,10 @@ lemma lMap_bind (b : Fin n₁ → Subterm L₁ μ₂ n₂) (e : μ₁ → Subter
 lemma lMap_map (b : Fin n₁ → Fin n₂) (e : μ₁ → μ₂) (p) :
     lMap Φ ((Rew.map b e).hom p) = (Rew.map b e).hom (lMap Φ p) := lMap_bind _ _ _
 
+lemma lMap_rewrite (f : μ → Subterm L₁ μ n) (p : Subformula L₁ μ n) :
+    lMap Φ ((Rew.rewrite f).hom p) = (Rew.rewrite (Subterm.lMap Φ ∘ f)).hom (lMap Φ p) :=
+  by simp[Rew.rewrite, lMap_bind, Function.comp]
+
 lemma lMap_substs (w : Fin k → Subterm L₁ μ n) (p : Subformula L₁ μ k) :
     lMap Φ ((Rew.substs w).hom p) = (Rew.substs (Subterm.lMap Φ ∘ w)).hom (lMap Φ p) := lMap_bind _ _ _
 
@@ -820,7 +825,7 @@ variable (ω : Rew L μ₁ n₁ μ₂ n₂)
 lemma hom_operator (o : Operator L k) (v : Fin k → Subterm L μ₁ n₁) :
     ω.hom (o.operator v) = o.operator (fun i => ω (v i)) := by
   simp[Operator.operator, ←Rew.hom_comp_app]; congr 2
-  ext <;> simp[Rew.comp_app]; contradiction
+  ext x <;> simp[Rew.comp_app]; exact x.elim0'
 
 lemma hom_operator' (o : Operator L k) (v : Fin k → Subterm L μ₁ n₁) :
     ω.hom (o.operator v) = o.operator (ω ∘ v) := ω.hom_operator o v
